Bound.dfy
@@ -10,7 +10,7 @@ predicate  myBoundsOK(oo : Owner, mb : Bound)
 //next trial
  {
   && (flatten(oo) >= flatten(mb))
-  && (forall o <- oo :: o.ownerBound() >= flatten(mb))
+  && (forall o <- oo :: flatten(o.ownerBound()) >= flatten(mb))
 //  && (forall o <- oo ::( ((o.AMFB) >= flatten(mb))))
 //  && (forall o <- oo ::( (o.AMFX > {}) ==> ((o.AMFB+{o}) >= flatten(mb))))
   }
@@ -57,7 +57,7 @@ lemma testBounds4(oo : Owner, mb : Bound)
   requires flatten(oo) >= flatten(mb)
   requires AllReady(oo)
   requires AllReady(mb)
-  requires forall o <- oo :: o.AMFB+{o} >= flatten(mb)   //PLUSo
+  requires forall o <- oo :: flatten(o.ownerBound()) >= flatten(mb)
    ensures myBoundsOK(oo, mb)
   {}
 
@@ -68,7 +68,7 @@ lemma  {:isolate_assertions} {:timeLimit 20} testBounds5(oo : Owner, mb : Bound)
    ensures forall o <- oo :: (o.AMFB == o.AMFX)
   requires forall o <- oo :: o.AMFX >= flatten(mb)
    ensures forall o <- oo :: o.AMFB >= flatten(mb)
-
+  requires forall o <- oo :: flatten(o.ownerBound()) >= flatten(mb)
    ensures myBoundsOK(oo, mb)
   {
     // calc {
@@ -82,16 +82,24 @@ lemma  {:isolate_assertions} {:timeLimit 20} testBounds5(oo : Owner, mb : Bound)
 
 
 
-lemma testBounds6(oo : Owner, mb : Bound, o : Object, b : Bound)
+lemma {:isolate_assertions} testBounds6(oo : Owner, mb : Bound, o : Object, b : Bound)
   requires AllReady(oo)
   requires AllReady(mb)
   requires oo == {o}   //singleton
-  requires mb == o.bound
+  requires mb == o.ownerBound()
+  requires flatten(oo) >= flatten(mb)
    ensures isFlat(o.AMFB)
    ensures (set o <- oo, ooo <- o.AMFB :: ooo ) == o.AMFB == flatten(o.bound)
-   ensures forall o <- oo :: o.AMFB >= flatten(mb)
+//   ensures forall o <- oo :: o.AMFB >= flatten(mb)
+   ensures forall o <- oo :: flatten(o.ownerBound()) >= flatten(mb)
    ensures myBoundsOK(oo, mb)
-  {}
+  {
+    assert mb == o.ownerBound();
+    assert forall o <- oo :: o.ownerBound() == mb;
+    assert forall o <- oo :: flatten(o.ownerBound()) == flatten(mb);
+
+
+  }
 
 lemma testBounds10(oo : Owner, mb : Bound)
     requires AllReady(oo)
@@ -102,7 +110,7 @@ lemma testBounds10(oo : Owner, mb : Bound)
 lemma testBounds11(oo : Owner, mb : Bound)
     requires flatten(oo) >= flatten(mb)
     requires AllReady(oo)
-    requires forall b <- flatten(mb), o <- oo :: b in o.AMFB+{o} //PLUSo
+    requires forall o <- oo :: flatten(o.ownerBound())>= flatten(mb)
      ensures forall o <- oo :: (o.AMFB+{o}) >= flatten(mb)   ///how come no PLUSo????
      ensures(forall o <- oo :: ((o.AMFX > {}) ==> ((o.AMFB+{o}) >= flatten(mb))))
      ensures myBoundsOK(oo, mb)
@@ -133,39 +141,77 @@ lemma testBounds13(a : Object, b : Object, c : Object, d : Object)
 
 
 
-lemma testBounds14(a : Object, b : Object, c : Object, d : Object)
-//simple row
-     requires c.AMFB == {a}
-     requires c.AMFO == {c,b,a}
+lemma {:isolate_assertions} testBounds14(a : Object, b : Object, c : Object)
+//learning from this method - setup owner and bound, NOT AMFX and friends...
+     requires a.Ready() && b.Ready() && c.Ready()
+      ensures c.AMFB == {a}
+      ensures c.AMFO == {c,b,a}
+     requires c.owner == {b}
+     requires c.bound == {a}
      requires b.AMFB == {a}
      requires b.AMFO == {a,b}
+      ensures b.owner == {a}
+      ensures b.bound == {a}
      requires a.AMFB == {}
      requires a.AMFO == {a}
-      ensures myBoundsOK( {c,b}, {a})
+      ensures myBoundsOK( {}, {})    //a
+      ensures myBoundsOK( {a}, {a})  //b
+      ensures myBoundsOK( {b}, {a})  //c
+      ensures myBoundsOK( {b}, {} )  //c?
+
       {
         assert flatten( {a} ) == {a};
+        assert flatten( {b} ) == {a,b};
+        assert flatten( {c} ) == {a,b,c};
+
+        assert flatten({}) >= flatten({});
+        assert flatten({b}) >= flatten({a});
+        assert flatten({c}) >= flatten({a});
+
+        assert a.ownerBound() == {a};
+
+        assert b.owner == {a};
+        assert b.bound == {a};
+        assert b.owner == b.bound;
+        assert b.ownerBound() == {b};
+
+        assert c.bound == {a};
+        assert c.ownerBound() == {a};
       }
 
 
 
-lemma testBounds15(a : Object, b : Object, c : Object, d : Object)
+lemma testBounds15(a : Object, b : Object, c : Object)
 //simple row
-     requires c.AMFB == {b,a}
-     requires c.AMFO == {b,a,c}
-     requires b.AMFB == {a}
-     requires b.AMFO == {b,a}
-     requires a.AMFB == {}
-     requires a.AMFX == {}
-     requires a.Ready()
-      ensures a.AMFO == {a}
+     requires a.Ready() && b.Ready() && c.Ready()
+     requires c.bound == {b}
+     requires c.owner == {b}
+     requires b.bound == {a}
+     requires b.owner == {a}
+     requires a.bound == {}
+     requires a.owner == {}
       ensures flatten({a}) == {a}
       ensures myBoundsOK( {c,b}, {a})
-      {
-        // assert {b,a} >= {a};
-        // assert {a} >= {a};
-        // assert c.AMFB >= flatten({a});
-      }
+      ensures myBoundsOK( {b},   {a})
+      ensures myBoundsOK( {c},   {a})
+      ensures myBoundsOK( {c},   {b})
+  { }
 
+
+lemma testBounds16(a : Object, b : Object, c : Object)
+//less simple row
+     requires a.Ready() && b.Ready() && c.Ready()
+     requires c.bound == {a}
+     requires c.owner == {b}
+     requires b.bound == {a}
+     requires b.owner == {a}
+     requires a.bound == {}
+     requires a.owner == {}
+      ensures flatten({a}) == {a}
+      ensures myBoundsOK( {c,b}, {a})
+      ensures myBoundsOK( {b},   {a})
+      ensures myBoundsOK( {c},   {a})
+  { }
 
 
 //////////////////////////////////////////////////////////////////////
@@ -175,8 +221,7 @@ lemma testBounds15(a : Object, b : Object, c : Object, d : Object)
 ///////
 
 method proposeBoundsFLAT(os : set<Object>) returns (b : Bound)
- //computes the intersection of the *flattened* bounds of each owner
- //does it?  are we sure?
+ //computes the intersection of the *flattened* bounds of each owner in os...
   requires AllReady(os)
    ensures myBoundsOK(os, b)
  {
@@ -185,16 +230,16 @@ method proposeBoundsFLAT(os : set<Object>) returns (b : Bound)
  }
 
 
-method opposeBounds(os : set<Object>) returns (b : Bound)
+method {:isolate_assertions}  opposeBounds(os : set<Object>) returns (b : Bound)
  //computes the intersection of the nominal bounds of each owner
  //does it?  are we sure?
+ //keeping it around because a) paranoia & b) "opposeBounds" is a funny name...
   requires AllReady(os)
    ensures myBoundsOK(os, b)
    ensures b == proposeBounds(os)
-   ensures myBoundsOK(os, b)
  {
-    var all : set<Object> := set o <- os, a <- o.bound :: a;
-    b := set a <- all | forall o <- os :: a in o.AMFB;
+    var all : set<Object> := set o <- os, a <- o.ownerBound() :: a;
+    b := set a <- all | forall o <- os :: flatten({a}) <= flatten(o.ownerBound());
  }
 
  function proposeBounds(os : set<Object>) : (b : Bound)
@@ -202,9 +247,25 @@ method opposeBounds(os : set<Object>) returns (b : Bound)
   requires AllReady(os)
    ensures myBoundsOK(os, b)
  {
-    var all : set<Object> := set o <- os, a <- o.bound :: a;
-    set a <- all | forall o <- os :: a in o.AMFB
+    var all : set<Object> := set o <- os, a <- o.ownerBound() :: a;
+    set a <- all | forall o <- os :: flatten({a}) <= flatten(o.ownerBound())
+
+   //set a <- all | forall o <- os :: a in flatten(o.ownerBound())
+ // set a <- all | forall o <- os :: flatten({a}) <= flatten(o.ownerBound())
+ //   set a <- all | forall o <- os :: flatten(o.ownerBound()) >= a.AMFO
+
  }
+//
+// lemma SAME_SAME_BOUNDS(os : set<Object>, all : set<Object>)
+//   requires AllReady(os)
+//   requires all == set o <- os, a <- o.ownerBound() :: a
+// //   ensures myBoundsOK(os, (set a <- all | forall o <- os :: a in flatten(o.ownerBound())))
+//   // ensures myBoundsOK(os, (set a <- all | forall o <- os :: a in o.ownerBound()))
+//  //  ensures myBoundsOK(os, (set a <- all | forall o <- os :: a.AMFO >= flatten(o.ownerBound())))
+//    ensures myBoundsOK(os, set a <- all | forall o <- os :: flatten({a}) <= flatten(o.ownerBound()))
+//    ensures myBoundsOK(os, set a <- all | forall o <- os :: flatten(o.ownerBound()) >= flatten({a}))
+//    {
+//    }
 
 
  function froposeBounds(os : set<Object>) : (b : Bound)
@@ -214,8 +275,9 @@ method opposeBounds(os : set<Object>) returns (b : Bound)
  //but can't guarantee anything
 //   ensures myBoundsOK(os, b)
  {
-    var all : set<Object> := set o <- os, a <- o.bound :: a;
-    set a <- all | forall o <- os :: a in (o.AMFB)
+    var all : set<Object> := set o <- os, a <- o.ownerBound() :: a;
+  //  set a <- all | forall o <- os :: flatten({a}) <= flatten(o.ownerBound())
+    set a <- all | forall o <- os ::  flatten(o.ownerBound()) >= flatten({a})
  }
 
 lemma {:isolate_assertions} froposeGetsBoundsOK(os : set<Object>, fp  : set<Object>)
@@ -227,10 +289,70 @@ lemma {:isolate_assertions} froposeGetsBoundsOK(os : set<Object>, fp  : set<Obje
      ensures myBoundsOK(os, fp)
 {}
 
+lemma {:isolate_assertions} OneNilOwner(a : Object)
+  requires a.Ready()
+  requires exists o : Object <- a.owner :: o.ownerBound() == {}
+   ensures a.bound == {}
+{
+  assert myBoundsOK(a.owner, a.bound);
+  assert forall o <- a.owner :: flatten(o.ownerBound()) >= flatten(a.bound);
+  assert flatten( {} ) == {};
+  assert exists o : Object <- a.owner :: o.ownerBound() == {};
+  assert exists o : Object <- a.owner :: flatten(o.ownerBound()) == {};
+  assert {} >= flatten(a.bound);
+  assert {} >= flatten(a.bound);
+  assert {} ==        (a.bound);
+}
+
+
+lemma {:isolate_assertions} OneNilAMFO(a : Object, o : Object)
+  decreases a.AMFO
+  requires a.Ready()
+  requires o in a.AMFO
+  requires o.ownerBound() == {}
+   ensures a.bound == {}
+{
+  if (o == a) { return; }
+  assert o != a;
+
+  if (o in a.owner) { OneNilOwner(a); return;  }
+  assert o !in a.owner;
+
+  assert exists x <- a.owner ::  o in x.AMFO;
+  var next :| (next in a.owner) && (o in next.AMFO);
+  OneNilAMFO(next, o);
+  assert next.bound == {};
+  OneNilOwner(a);
+  assert a.bound == {};
+}
+
 
 //////////////////////////////////////////////////////////////////////
+lemma {:isolate_assertions} TransitiveBounds(part : Object,  whole : Object)
+ decreases part.AMFO
+  requires part.Ready() && whole.Ready()
+  requires inside(part,whole)
+   ensures myBoundsOK(part.owner, part.bound)
+   ensures myBoundsOK(whole.owner, whole.bound)
+   ensures part.AMFO >=  whole.AMFO
+   ensures part.AMFO  > part.AMFB
+   ensures whole.AMFO > whole.AMFB
+//   ensures part.AMFB >= whole.AMFB
+   ensures (forall o <- part.owner  :: flatten(o.ownerBound()) >= part.AMFB)
+   ensures (forall o <- whole.owner :: flatten(o.ownerBound()) >= whole.AMFB)
+  ensures forall o <- whole.owner ::( (o.AMFX > {}) ==> ((o.AMFB+{o}) >= whole.AMFB))
+//   ensures (forall o <- part.owner  :: flatten(o.ownerBound()) >= whole.AMFB)
+{
+ InsideRecInside2(part, whole);
+     assert myBoundsOK(part.owner, part.bound);
+       assert (flatten(part.owner) >= flatten(part.bound));
+       assert (forall o <- part.owner ::( (o.AMFX > {}) ==> ((o.AMFB+{o}) >= flatten(part.bound))));
 
-lemma {:isolate_assertions} {:timeLimit 30} TransitiveBounds(part : Object,  whole : Object)
+    if  ((part == whole) || (whole in part.owner)) { return; }
+
+}
+
+lemma {:isolate_assertions} {:verify false} OLD_TransitiveBounds(part : Object,  whole : Object)
  /// warning - this reqhires SingleOwnership ie is BAD
  decreases part.AMFO
   requires part.Ready() && whole.Ready()
